lazy_list/client.v
@@ -1,0 +1,126 @@
+From Coq Require Import Lia.
+
+From iris.heap_lang Require Import notation par proofmode.
+From iris.algebra Require Import frac.
+
+From SkipList.lib Require Import lock misc.
+From SkipList.lazy_list Require Import code.
+From SkipList.lazy_list.inv Require Import list_equiv inv.
+From SkipList.lazy_list.spec Require Import new contains add.
+
+
+Local Open Scope Z.
+
+Module Params <: LAZY_LIST_PARAMS.
+  Definition INT_MIN := -1000.
+  Definition INT_MAX := 1000.
+  Lemma HMIN_MAX : INT_MIN < INT_MAX.
+  Proof. unfold INT_MIN, INT_MAX; lia. Qed.
+End Params.
+
+Module Import New := NewSpec Params.
+Module Import Contains := ContainsSpec Params.
+Module Import Add := AddSpec Params.
+
+(* Convert a list of Coq ints into a HeapLang tuple *)
+Fixpoint L2tuple (L: list Z) : val :=
+  match L with
+  | nil => NONEV
+  | z :: L =>
+    SOMEV (#z, L2tuple L)
+  end.
+
+Definition addList : val :=
+  rec: "add" "lazy" "L" :=
+    match: "L" with
+      NONE => #()
+    | SOME "pair" =>
+      let: "key" := Fst "pair" in
+      let: "tail" := Snd "pair" in
+        add "lazy" "key";;
+        "add" "lazy" "tail"
+    end.
+
+Definition lazy_list_client (L1 L2: list Z) (key: Z) : expr := 
+  let: "lazy" := new #() in
+    (addList "lazy" (L2tuple L1) ||| addList "lazy" (L2tuple L2));;
+    contains "lazy" #key.
+
+Section Proofs.
+  Context `{!heapGS Σ, !gset_list_unionGS Σ, !lockG Σ, !spawnG Σ}.
+
+  Lemma addList_spec (v: val) (S: gset Z) (q: frac) (Γ: lazy_gname) (L: list Z) :
+    (∀ (k: Z), k ∈ L → Params.INT_MIN < k < Params.INT_MAX) →
+    {{{ is_lazy_list v S q Γ }}}
+      addList v (L2tuple L)
+    {{{ RET #(); is_lazy_list v (set_list_union S L) q Γ }}}.
+  Proof.
+    iIntros (Hrange Φ) "Hlazy HΦ".
+    iRevert (S L Hrange) "Hlazy HΦ".
+    iLöb as "IH".
+    iIntros (S L Hrange) "Hlazy HΦ".
+
+    wp_lam. wp_let.
+    destruct L as [|key L]; wp_match.
+    + iModIntro. iApply "HΦ". iFrame.
+    + wp_pures.
+      wp_apply (add_spec with "Hlazy").
+      { apply Hrange. left. }
+
+      iIntros (b) "Hlazy".
+      wp_pures.
+      iApply ("IH" with "[%] [$]").
+      { intros k Hin. apply Hrange. by right. }
+
+      iNext; iFrame.
+  Qed.
+
+  Lemma lazy_list_client_spec (L1 L2: list Z) (key: Z) :
+    (Params.INT_MIN < key < Params.INT_MAX) →
+    (∀ (k: Z), k ∈ L1 ∨ k ∈ L2 → Params.INT_MIN < k < Params.INT_MAX) →
+    {{{ True }}}
+      lazy_list_client L1 L2 key
+    {{{ (b: bool), RET #b;
+      ⌜ if b then key ∈ L1 ∨ key ∈ L2 
+             else key ∉ L1 ∧ key ∉ L2 ⌝ 
+    }}}.
+  Proof.
+    iIntros (Hrange Hrange_l Φ) "_ HΦ".
+
+    unfold lazy_list_client.
+    wp_apply new_spec; first done.
+    iIntros (v Γ) "Hlazy".
+
+    wp_let.
+    rewrite -(Qp_div_2 1).
+    iDestruct (is_lazy_list_sep with "Hlazy") as "(Hlazy1 & Hlazy2)".
+
+    wp_smart_apply (wp_par (λ _, is_lazy_list v (set_list_union ∅ L1) (1 / 2) Γ)
+                           (λ _, is_lazy_list v (set_list_union ∅ L2) (1 / 2) Γ) 
+                           with "[Hlazy1] [Hlazy2]").
+    + wp_apply (addList_spec with "Hlazy1").
+      { intros k Hin. apply Hrange_l. by left. }
+      by iIntros.
+    + wp_apply (addList_spec with "Hlazy2").
+      { intros k Hin. apply Hrange_l. by right. }
+      by iIntros.
+    + iIntros (v1 v2) "Hlazy".
+      rewrite is_lazy_list_join (Qp_div_2 1).
+      
+      iNext; wp_pures.
+      wp_apply (contains_spec with "Hlazy"); first done.
+      iIntros (b) "(Hlazy & %Hif)".
+      iApply "HΦ". iPureIntro. 
+      
+      destruct b.
+      - rewrite elem_of_union in Hif.
+        destruct Hif as [Hin1 | Hin2].
+        * left. by apply in_empty_set_list_union.
+        * right. by apply in_empty_set_list_union.
+      - rewrite elem_of_union in Hif.
+        split; intros Hfalse; destruct Hif.
+        * left. by apply in_empty_set_list_union.
+        * right. by apply in_empty_set_list_union.
+  Qed.
+
+End Proofs.
