lazy_list/code.v
@@ -2,6 +2,7 @@ From SkipList.lib Require Import lock node_rep.
 
 
 Local Open Scope Z.
+
 Module Type LAZY_LIST_PARAMS.
   Parameter INT_MIN : Z.
   Parameter INT_MAX : Z.
@@ -17,37 +18,37 @@ Module LazyList (Params: LAZY_LIST_PARAMS).
     rec: "find" "pred" "k" :=
       let: "ocurr" := (nodeNext "pred") in
       match: "ocurr" with
-          NONE => NONEV
-        | SOME "np" => 
-          let: "curr" := !"np" in
-          let: "ck" := (nodeKey "curr") in
-          if: "k" ≤ "ck"
-          then SOME ("pred", "curr")
-          else "find" "curr" "k"
+        NONE => NONEV
+      | SOME "np" => 
+        let: "curr" := !"np" in
+        let: "ck" := (nodeKey "curr") in
+        if: "k" ≤ "ck"
+        then SOME ("pred", "curr")
+        else "find" "curr" "k"
       end.
   
   Definition findLock : val := 
     rec: "find" "head" "k" :=
       let: "opair" := find "head" "k" in
       match: "opair" with
+        NONE => NONEV
+      | SOME "pair" =>
+        let: "pred" := Fst "pair" in
+        let: "curr" := Snd "pair" in
+        acquire (nodeLock "pred");;
+        let: "onext" := (nodeNext "pred") in
+        match: "onext" with
           NONE => NONEV
-        | SOME "pair" =>
-          let: "pred" := Fst "pair" in
-          let: "curr" := Snd "pair" in
-          acquire (nodeLock "pred");;
-          let: "onext" := (nodeNext "pred") in
-          match: "onext" with
-              NONE => NONEV
-            | SOME "np" =>
-              let: "next" := !"np" in
-              let: "nk" := (nodeKey "next") in
-              let: "ck" := (nodeKey "curr") in
-              if: "nk" = "ck" 
-              then SOME ("pred", "curr")
-              else
-                release (nodeLock "pred");;
-                "find" "pred" "k"
-          end
+        | SOME "np" =>
+          let: "next" := !"np" in
+          let: "nk" := (nodeKey "next") in
+          let: "ck" := (nodeKey "curr") in
+          if: "nk" = "ck" 
+          then SOME ("pred", "curr")
+          else
+            release (nodeLock "pred");;
+            "find" "pred" "k"
+        end
       end.
   
   Definition dummy_lock : val := #{|loc_car := 0|}.
@@ -64,11 +65,11 @@ Module LazyList (Params: LAZY_LIST_PARAMS).
     λ: "head" "k",
       let: "opair" := find !"head" "k" in
       match: "opair" with
-          NONE => #false
-        | SOME "pair" =>
-          let: "curr" := Snd "pair" in
-          let: "ck" := (nodeKey "curr") in
-          ("k" = "ck") 
+        NONE => #false
+      | SOME "pair" =>
+        let: "curr" := Snd "pair" in
+        let: "ck" := (nodeKey "curr") in
+        ("k" = "ck") 
       end.
   
   (* Lazy list insertion *)
@@ -76,28 +77,28 @@ Module LazyList (Params: LAZY_LIST_PARAMS).
     λ: "head" "k",
       let: "opair" := findLock !"head" "k" in
       match: "opair" with
-          NONE => #false
-        | SOME "pair" =>
-          let: "pred" := Fst "pair" in
-          let: "curr" := Snd "pair" in
-          let: "ck" := (nodeKey "curr") in
-          if: "k" = "ck"
-          then
+        NONE => #false
+      | SOME "pair" =>
+        let: "pred" := Fst "pair" in
+        let: "curr" := Snd "pair" in
+        let: "ck" := (nodeKey "curr") in
+        if: "k" = "ck"
+        then
+          release (nodeLock "pred");;
+          #false
+        else
+          match: nodeNext "pred" with
+            NONE =>
             release (nodeLock "pred");;
             #false
-          else
-            match: nodeNext "pred" with
-                NONE =>
-                release (nodeLock "pred");;
-                #false
-              | SOME "np" =>
-                let: "succ" := !"np" in
-                let: "next" := ref "succ" in
-                let: "node" := ("k", SOME "next", NONEV, newlock #()) in
-                "np" <- "node";;
-                release (nodeLock "pred");;
-                #true
-            end
+          | SOME "np" =>
+            let: "succ" := !"np" in
+            let: "next" := ref "succ" in
+            let: "node" := ("k", SOME "next", NONEV, newlock #()) in
+            "np" <- "node";;
+            release (nodeLock "pred");;
+            #true
+          end
       end.
 
 End LazyList.
