skip_list/client.v
@@ -1,0 +1,139 @@
+From Coq Require Import Lia.
+
+From iris.heap_lang Require Import notation par proofmode.
+From iris.algebra Require Import frac.
+
+From SkipList.lib Require Import lock misc.
+From SkipList.skip_list Require Import code.
+From SkipList.skip_list.inv Require Import list_equiv lazy_inv skip_inv.
+From SkipList.skip_list.spec Require Import new contains add.
+
+
+Local Open Scope Z.
+
+Module Params <: SKIP_LIST_PARAMS.
+  Definition INT_MIN := -1000.
+  Definition INT_MAX := 1000.
+  Definition MAX_HEIGHT := 20.  
+  Lemma HMIN_MAX : INT_MIN < INT_MAX.
+  Proof. unfold INT_MIN, INT_MAX; lia. Qed.
+End Params.
+
+Module Import New := NewSpec Params.
+Module Import Contains := ContainsSpec Params.
+Module Import Add := AddSpec Params.
+
+Notation node := (prod Z Z).
+Definition keys (L: list node) : list Z := map fst L.
+Definition heights (L: list node) : list Z := map snd L.
+
+(* Convert a list of Coq ints into a HeapLang tuple *)
+Fixpoint L2tuple (L: list node) : val :=
+  match L with
+  | nil => NONEV
+  | (z, h) :: L => SOMEV (#z, #h, L2tuple L)
+  end.
+
+Definition addList : val :=
+  rec: "add" "skip" "L" :=
+    match: "L" with
+      NONE => #()
+    | SOME "tuple" =>
+      let: "key" := Fst (Fst "tuple") in
+      let: "height" := Snd (Fst "tuple") in
+      let: "tail" := Snd "tuple" in
+        add "skip" "key" "height";;
+        "add" "skip" "tail"
+    end.
+
+Definition skip_list_client (L1 L2: list node) (key: Z) : expr := 
+  let: "skip" := new #() in
+    (addList "skip" (L2tuple L1) ||| addList "skip" (L2tuple L2));;
+    contains "skip" #key.
+
+Section Proofs.
+  Context `{!heapGS Σ, !gset_list_unionGS Σ, !lockG Σ, !spawnG Σ}.
+
+  Lemma addList_spec (v: val) (S: gset Z) (q: frac) 
+    (bot: bot_gname) (subs: list sub_gname) (L: list node) :
+    (∀ (k: Z), k ∈ keys L → Params.INT_MIN < k < Params.INT_MAX) →
+    (∀ (h: Z), h ∈ heights L → 1 ≤ h ≤ Params.MAX_HEIGHT) →
+    {{{ is_skip_list v S q bot subs }}}
+      addList v (L2tuple L)
+    {{{ RET #(); is_skip_list v (set_list_union S (keys L)) q bot subs }}}.
+  Proof.
+    iIntros (Hk_range Hh_range Φ) "Hskip HΦ".
+    iRevert (S L Hk_range Hh_range) "Hskip HΦ".
+    iLöb as "IH".
+    iIntros (S L Hk_range Hh_range) "Hskip HΦ".
+
+    wp_lam. wp_let.
+    destruct L as [|pair L].
+    + wp_match. iModIntro. iApply "HΦ". iFrame.
+    + destruct pair as [key height]. wp_pures. 
+      
+      wp_apply (add_spec with "Hskip").
+      { apply Hk_range. left. }
+      { apply Hh_range. left. }
+
+      iIntros (b) "Hskip".
+      wp_pures.
+      iApply ("IH" with "[%] [%] [$]").
+      { intros k Hin. apply Hk_range. by right. }
+      { intros h Hin. apply Hh_range. by right. }
+
+      iNext; iFrame.
+  Qed.
+
+  Lemma skip_list_client_spec (L1 L2: list node) (key: Z) :
+    (Params.INT_MIN < key < Params.INT_MAX) →
+    (∀ (k: Z), k ∈ keys L1 ∨ k ∈ keys L2 → Params.INT_MIN < k < Params.INT_MAX) →
+    (∀ (h: Z), h ∈ heights L1 ∨ h ∈ heights L2 → 1 ≤ h ≤ Params.MAX_HEIGHT) →
+    {{{ True }}}
+      skip_list_client L1 L2 key
+    {{{ (b: bool), RET #b;
+      ⌜ if b then key ∈ keys L1 ∨ key ∈ keys L2 
+             else key ∉ keys L1 ∧ key ∉ keys L2 ⌝ 
+    }}}.
+  Proof.
+    iIntros (Hrange Hk_range Hh_range Φ) "_ HΦ".
+
+    unfold skip_list_client.
+    wp_apply new_spec; first done.
+    iIntros (v bot subs) "Hskip".
+
+    wp_let.
+    rewrite -(Qp_div_2 1).
+    iDestruct (is_skip_list_sep with "Hskip") as "(Hskip1 & Hskip2)".
+
+    wp_smart_apply (wp_par (λ _, is_skip_list v (set_list_union ∅ (keys L1)) (1 / 2) bot subs)
+                           (λ _, is_skip_list v (set_list_union ∅ (keys L2)) (1 / 2) bot subs) 
+                           with "[Hskip1] [Hskip2]").
+    + wp_apply (addList_spec with "Hskip1").
+      { intros k Hin. apply Hk_range. by left. }
+      { intros h Hin. apply Hh_range. by left. }
+      by iIntros.
+    + wp_apply (addList_spec with "Hskip2").
+      { intros k Hin. apply Hk_range. by right. }
+      { intros h Hin. apply Hh_range. by right. }
+      by iIntros.
+    + iIntros (v1 v2) "Hskip".
+      rewrite is_skip_list_join (Qp_div_2 1).
+      
+      iNext; wp_pures.
+      wp_apply (contains_spec with "Hskip"); first done.
+      iIntros (b) "(Hskip & %Hif)".
+      iApply "HΦ". iPureIntro. 
+      
+      destruct b.
+      - rewrite elem_of_union in Hif.
+        destruct Hif as [Hin1 | Hin2].
+        * left. by apply in_empty_set_list_union.
+        * right. by apply in_empty_set_list_union.
+      - rewrite elem_of_union in Hif.
+        split; intros Hfalse; destruct Hif.
+        * left. by apply in_empty_set_list_union.
+        * right. by apply in_empty_set_list_union.
+  Qed.
+
+End Proofs.
