skip_list/code.v
@@ -2,6 +2,7 @@ From SkipList.lib Require Import lock node_rep.
 
 
 Local Open Scope Z.
+
 Module Type SKIP_LIST_PARAMS.
   Parameter INT_MIN : Z.
   Parameter INT_MAX : Z.
@@ -43,37 +44,37 @@ Module SkipList (Params: SKIP_LIST_PARAMS).
     rec: "find" "pred" "k" :=
       let: "ocurr" := (nodeNext "pred") in
       match: "ocurr" with
-          NONE => NONEV
-        | SOME "np" => 
-          let: "curr" := !"np" in
-          let: "ck" := (nodeKey "curr") in
-          if: "k" ≤ "ck"
-          then SOME ("pred", "curr")
-          else "find" "curr" "k"
+        NONE => NONEV
+      | SOME "np" => 
+        let: "curr" := !"np" in
+        let: "ck" := (nodeKey "curr") in
+        if: "k" ≤ "ck"
+        then SOME ("pred", "curr")
+        else "find" "curr" "k"
       end.
   
   Definition findLock : val := 
     rec: "find" "head" "k" :=
       let: "opair" := find "head" "k" in
       match: "opair" with
+        NONE => NONEV
+      | SOME "pair" =>
+        let: "pred" := Fst "pair" in
+        let: "curr" := Snd "pair" in
+        acquire (nodeLock "pred");;
+        let: "onext" := (nodeNext "pred") in
+        match: "onext" with
           NONE => NONEV
-        | SOME "pair" =>
-          let: "pred" := Fst "pair" in
-          let: "curr" := Snd "pair" in
-          acquire (nodeLock "pred");;
-          let: "onext" := (nodeNext "pred") in
-          match: "onext" with
-              NONE => NONEV
-            | SOME "np" =>
-              let: "next" := !"np" in
-              let: "nk" := (nodeKey "next") in
-              let: "ck" := (nodeKey "curr") in
-              if: "nk" = "ck" 
-              then SOME ("pred", "curr")
-              else
-                release (nodeLock "pred");;
-                "find" "pred" "k"
-          end
+        | SOME "np" =>
+          let: "next" := !"np" in
+          let: "nk" := (nodeKey "next") in
+          let: "ck" := (nodeKey "curr") in
+          if: "nk" = "ck" 
+          then SOME ("pred", "curr")
+          else
+            release (nodeLock "pred");;
+            "find" "pred" "k"
+        end
       end.
 
   (* Lazy list lookup *)
@@ -81,71 +82,71 @@ Module SkipList (Params: SKIP_LIST_PARAMS).
     rec: "find" "head" "k" := 
       let: "opair" := find "head" "k" in
       match: "opair" with
-          NONE => NONEV
-        | SOME "pair" =>
-          let: "pred" := Fst "pair" in
-          let: "curr" := Snd "pair" in
-          match: nodeDown "pred" with
-              NONE => SOME ("pred", "curr")
-            | SOME "np" => 
-              let: "pred" := !"np" in
-              "find" "pred" "k"
-          end
+        NONE => NONEV
+      | SOME "pair" =>
+        let: "pred" := Fst "pair" in
+        let: "curr" := Snd "pair" in
+        match: nodeDown "pred" with
+          NONE => SOME ("pred", "curr")
+        | SOME "np" => 
+          let: "pred" := !"np" in
+          "find" "pred" "k"
+        end
       end.
 
   Definition contains : val := 
     λ: "head" "k", 
       let: "opair" := findPred !"head" "k" in
       match: "opair" with
-          NONE => #false
-        | SOME "pair" => 
-          let: "curr" := Snd "pair" in
-          let: "ck" := nodeKey "curr" in
-          "k" = "ck"
+        NONE => #false
+      | SOME "pair" => 
+        let: "curr" := Snd "pair" in
+        let: "ck" := nodeKey "curr" in
+        "k" = "ck"
       end.
 
   (* Lazy list insertion *)
   Definition link : val := 
     λ: "pred" "k" "odown",
       match: nodeNext "pred" with
-          NONE => 
-          release (nodeLock "pred");;
-          NONEV
-        | SOME "np" =>
-          let: "succ" := !"np" in
-          let: "next" := ref "succ" in
-          let: "node" := ("k", SOME "next", "odown", newlock #()) in
-          "np" <- "node";;
-          release (nodeLock "pred");;
-          SOME "node"
+        NONE => 
+        release (nodeLock "pred");;
+        NONEV
+      | SOME "np" =>
+        let: "succ" := !"np" in
+        let: "next" := ref "succ" in
+        let: "node" := ("k", SOME "next", "odown", newlock #()) in
+        "np" <- "node";;
+        release (nodeLock "pred");;
+        SOME "node"
       end.
 
   Definition tryInsert : val := 
     λ: "head" "k",
       let: "opair" := findLock "head" "k" in
       match: "opair" with
-          NONE => NONEV
-        | SOME "pair" =>
-          let: "pred" := Fst "pair" in
-          let: "curr" := Snd "pair" in
-          let: "ck" := (nodeKey "curr") in
-          if: "k" = "ck"
-          then
-            release (nodeLock "pred");;
-            NONEV
-          else
-            link "pred" "k" NONEV
+        NONE => NONEV
+      | SOME "pair" =>
+        let: "pred" := Fst "pair" in
+        let: "curr" := Snd "pair" in
+        let: "ck" := (nodeKey "curr") in
+        if: "k" = "ck"
+        then
+          release (nodeLock "pred");;
+          NONEV
+        else
+          link "pred" "k" NONEV
       end.
 
   Definition insert : val := 
     λ: "head" "k" "down",
       let: "opair" := findLock "head" "k" in
       match: "opair" with
-          NONE => NONEV
-        | SOME "pair" =>
-          let: "pred" := Fst "pair" in
-          let: "d" := ref "down" in
-          link "pred" "k" (SOME "d")
+        NONE => NONEV
+      | SOME "pair" =>
+        let: "pred" := Fst "pair" in
+        let: "d" := ref "down" in
+        link "pred" "k" (SOME "d")
       end.
 
   (* Skip list insertion *)
@@ -153,50 +154,50 @@ Module SkipList (Params: SKIP_LIST_PARAMS).
     rec: "loop" "head" "k" "h" "l" :=
       let: "opair" := find "head" "k" in
       match: "opair" with
-          NONE => NONEV
-        | SOME "pair" =>
-          let: "pred" := Fst "pair" in
-          if: "h" = "l"
-          then SOME "pred"
-          else
-            match: nodeDown "pred" with
-                NONE => NONEV
-              | SOME "np" => 
-                let: "pred" := !"np" in
-                "loop" "pred" "k" "h" ("l" - #1)
-            end
+        NONE => NONEV
+      | SOME "pair" =>
+        let: "pred" := Fst "pair" in
+        if: "h" = "l"
+        then SOME "pred"
+        else
+          match: nodeDown "pred" with
+            NONE => NONEV
+          | SOME "np" => 
+            let: "pred" := !"np" in
+            "loop" "pred" "k" "h" ("l" - #1)
+          end
       end.
       
   Definition addAll : val := 
     rec: "add" "head" "k" := 
       let: "opair" := find "head" "k" in
       match: "opair" with
-          NONE => NONEV
-        | SOME "pair" =>
-          let: "pred" := Fst "pair" in
-          match: nodeDown "pred" with
-              NONE => tryInsert "pred" "k"
-            | SOME "np" => 
-              let: "down" := !"np" in
-              let: "onode" := "add" "down" "k" in
-              match: "onode" with 
-                  NONE => NONEV
-                | SOME "node" => insert "pred" "k" "node"
-              end
+        NONE => NONEV
+      | SOME "pair" =>
+        let: "pred" := Fst "pair" in
+        match: nodeDown "pred" with
+          NONE => tryInsert "pred" "k"
+        | SOME "np" => 
+          let: "down" := !"np" in
+          let: "onode" := "add" "down" "k" in
+          match: "onode" with 
+            NONE => NONEV
+          | SOME "node" => insert "pred" "k" "node"
           end
+        end
       end.
 
   Definition add : val := 
     λ: "head" "k" "h",
       let: "opred" := topLevel !"head" "k" "h" #MAX_HEIGHT in
       match: "opred" with
+        NONE => #false
+      | SOME "pred" => 
+        let: "onew" := addAll "pred" "k" in
+        match: "onew" with
           NONE => #false
-        | SOME "pred" => 
-          let: "onew" := addAll "pred" "k" in
-          match: "onew" with
-              NONE => #false
-            | SOME "new" => #true
-          end
+        | SOME "new" => #true
+        end
       end.
 
 End SkipList.
